-

ocaml/puiseux_series.ml
@@ -1,4 +1,4 @@
-(* $Id: puiseux_series.ml,v 1.136 2013-06-12 15:19:40 deraugla Exp $ *)
+(* $Id: puiseux_series.ml,v 1.137 2013-06-12 15:27:26 deraugla Exp $ *)
 
 #load "./pa_coq.cmo";
 
@@ -95,7 +95,8 @@ Record fifo_elem α :=
   { fe_t₁ : term α; fe_t₂ : term α;
     fe_s₁ : series (term α); fe_s₂ : series (term α) };
 
-Fixpoint add_coeff_list α (add_coeff : α → α → α) mul_coeff c₁ fel₁ :=
+Fixpoint add_coeff_list α (add_coeff : α → α → α) (mul_coeff : α → α → α)
+    c₁ fel₁ :=
   match fel₁ with
   | [] =>
       c₁
@@ -134,7 +135,7 @@ Fixpoint insert_sum α sum (fe : fifo_elem α) sl :=
 Definition add_below α (mul_coeff : α → α → α) sl fel :=
   List.fold_left
     (λ sl₁ fe,
-       match fe_s₁ fe with
+       match (fe_s₁ fe : series (term α)) with
        | Term t₁ s₁ =>
             insert_sum (Qred (Qplus (power t₁) (power (fe_t₂ fe))))
               {| fe_t₁ := t₁; fe_t₂ := fe_t₂ fe;
@@ -147,7 +148,7 @@ Definition add_below α (mul_coeff : α → α → α) sl fel :=
 Definition add_right α (mul_coeff : α → α → α) sl fel :=
   List.fold_left
     (λ sl₂ fe,
-       match fe_s₂ fe with
+       match (fe_s₂ fe : series (term α)) with
        | Term t₂ s₂ =>
             insert_sum (Qred (Qplus (power (fe_t₁ fe)) (power t₂)))
               {| fe_t₁ := fe_t₁ fe; fe_t₂ := t₂;
@@ -173,7 +174,7 @@ CoFixpoint ps_mul_loop α add_coeff mul_coeff sum_fifo :
       Term m (ps_mul_loop add_coeff mul_coeff sl₂)
   end;
 
-Definition ps_mul_term α add_coeff (mul_coeff : α → α → α) s₁ s₂ cd₁ cd₂ :=
+Definition ps_mul_term α add_coeff (mul_coeff : α → α → α) s₁ s₂ :=
   match s₁ with
   | Term t₁ ns₁ =>
       match s₂ with
@@ -190,9 +191,9 @@ Definition ps_mul_term α add_coeff (mul_coeff : α → α → α) s₁ s₂ cd�
 
 Definition ps_mul α add_coeff mul_coeff (ps₁ ps₂ : puiseux_series α) :=
   {| ps_terms :=
-       ps_mul_term add_coeff mul_coeff (ps_terms ps₁) (ps_terms ps₂)
-         (ps_comden ps₁) (ps_comden ps₂);
-     ps_comden := Nat.lcm (ps_comden ps₁) (ps_comden ps₂) |};
+       ps_mul_term add_coeff mul_coeff (ps_terms ps₁) (ps_terms ps₂);
+     ps_comden :=
+       Nat.lcm (ps_comden ps₁) (ps_comden ps₂) |};
 
 (**)
 
